characteristic/cfScript.sml
@@ -1712,58 +1712,6 @@ Definition cf_xoraw8str_def:
       app_xoraw8str s d H Q)
 End
 
-Definition cf_wordFromInt_W8_def:
-  cf_wordFromInt_W8 xi = \env. local (\H Q.
-    ?i.
-      exp2v env xi = SOME (Litv (IntLit i)) /\
-      app_wordFromInt_W8 i H Q)
-End
-
-Definition cf_wordFromInt_W64_def:
-  cf_wordFromInt_W64 xi = \env. local (\H Q.
-    ?i.
-      exp2v env xi = SOME (Litv (IntLit i)) /\
-      app_wordFromInt_W64 i H Q)
-End
-
-Definition cf_wordToInt_W8_def:
-  cf_wordToInt_W8 xw = \env. local (\H Q.
-    ?w.
-      exp2v env xw = SOME (Litv (Word8 w)) /\
-      app_wordToInt w H Q)
-End
-
-Definition cf_wordToInt_W64_def:
-  cf_wordToInt_W64 xw = \env. local (\H Q.
-    ?w.
-      exp2v env xw = SOME (Litv (Word64 w)) /\
-      app_wordToInt w H Q)
-End
-
-Definition app_fptoword_def:
-   app_fptoword fp H Q =
-   (H ==>> Q (Val (Litv (Word64 fp))))
-End
-
-Definition cf_fptoword_def:
- cf_fptoword xd = λ env. local ( λ H Q.
-   ∃ fp.
-   exp2v env xd = SOME (Litv (Float64 fp)) ∧
-   app_fptoword fp H Q)
-End
-
-Definition app_fpfromword_def:
- app_fpfromword w H Q =
- (H ==>> Q (Val (Litv (Float64 w))))
-End
-
-Definition cf_fpfromword_def:
- cf_fpfromword xw = λ env. local (λ H Q.
-   ∃ w.
-   exp2v env xw = SOME (Litv (Word64 w)) ∧
-   app_fpfromword w H Q)
-End
-
 Definition app_ffi_def:
   app_ffi ffi_index c a H Q =
     ((?conf ws frame s u ns events.
@@ -1799,7 +1747,8 @@ Definition cf_log_def:
            (And, T) => cf2 env H Q
          | (Or, F) => cf2 env H Q
          | (Or, T) => (H ==>> Q (Val v))
-         | (And, F) => (H ==>> Q (Val v))))
+         | (And, F) => (H ==>> Q (Val v))
+         | _ => F))
 End
 
 Definition cf_if_def:
@@ -1947,33 +1896,9 @@ Definition cf_def:
           (case args of
              | [d; s] => cf_xoraw8str s d
              | _ => cf_bottom)
-        | WordFromInt W8 =>
-          (case args of
-             | [i] => cf_wordFromInt_W8 i
-             | _ => cf_bottom)
-        | WordFromInt W64 =>
-          (case args of
-             | [i] => cf_wordFromInt_W64 i
-             | _ => cf_bottom)
-        | WordToInt W8 =>
-          (case args of
-             | [w] => cf_wordToInt_W8 w
-             | _ => cf_bottom)
-        | WordToInt W64 =>
-          (case args of
-             | [w] => cf_wordToInt_W64 w
-             | _ => cf_bottom)
         | FFI ffi_index =>
           (case args of
              | [c;w] => cf_ffi ffi_index c w
-             | _ => cf_bottom)
-        | FpFromWord =>
-          (case args of
-             | [w] => cf_fpfromword w
-             | _ => cf_bottom)
-        | FpToWord =>
-          (case args of
-             | [w] => cf_fptoword w
              | _ => cf_bottom)
         | _ => cf_bottom) /\
   cf (p:'ffi ffi_proj) (Log lop e1 e2) =
@@ -2026,12 +1951,6 @@ val cf_defs = [
   cf_copystraw8_def,
   cf_copyaw8str_def,
   cf_xoraw8str_def,
-  cf_wordFromInt_W8_def,
-  cf_wordFromInt_W64_def,
-  cf_wordToInt_W8_def,
-  cf_wordToInt_W64_def,
-  cf_fpfromword_def,
-  cf_fptoword_def,
   cf_app_def,
   cf_ref_def,
   cf_assign_def,
@@ -2886,24 +2805,6 @@ Proof
       qexists_tac `{}` \\ fs [st2heap_def] \\ SPLIT_TAC
     )
     THEN1 (
-     (* FpFromWord *)
-     Q.REFINE_EXISTS_TAC ‘Val v’ \\ simp[] \\ cf_evaluate_step_tac
-     \\ simp[]
-     \\ progress SPLIT3_of_SPLIT_emp3 \\ instantiate
-     \\ GEN_EXISTS_TAC "ck" ‘st.clock’ \\ fs[with_clock_self]
-     \\ cf_exp2v_evaluate_tac ‘st’ \\ fs [do_app_def, app_fpfromword_def]
-     \\ fs [SEP_IMP_def]
-     \\ fs [state_component_equality])
-    THEN1 (
-     (* FpToWord *)
-     Q.REFINE_EXISTS_TAC ‘Val v’ \\ simp[] \\ cf_evaluate_step_tac
-     \\ simp[]
-     \\ progress SPLIT3_of_SPLIT_emp3 \\ instantiate
-     \\ GEN_EXISTS_TAC "ck" ‘st.clock’ \\ fs[with_clock_self]
-     \\ cf_exp2v_evaluate_tac ‘st’ \\ fs [do_app_def, app_fptoword_def]
-     \\ fs [SEP_IMP_def]
-     \\ fs [state_component_equality])
-    THEN1 (
       (* Opapp *)
       rename1 `dest_opapp _ = SOME (f, xs)` \\
       rpt (pop_assum mp_tac) \\ SPEC_ALL_TAC \\
@@ -3243,15 +3144,6 @@ Proof
       qexists_tac `{}` \\ mp_tac store2heap_IN_unique_key \\ rpt strip_tac
       THEN1 (progress_then (fs o sing) store2heap_LUPDATE \\ SPLIT_TAC)
       THEN1 (first_assum irule \\ instantiate \\ SPLIT_TAC)
-    ) \\
-    try_finally (
-      (* WordFromInt W8, WordFromInt W64, WordToInt W8, WordToInt W64 *)
-      Q.REFINE_EXISTS_TAC `Val v` \\ simp [] \\ cf_evaluate_step_tac \\
-      GEN_EXISTS_TAC "ck" `st.clock` \\ fs [with_clock_self] \\
-      cf_exp2v_evaluate_tac `st` \\ fs [do_app_def] \\
-      fs [app_wordFromInt_W8_def, app_wordFromInt_W64_def, app_wordToInt_def] \\
-      fs [SEP_IMP_def, st2heap_def] \\ res_tac \\
-      progress SPLIT3_of_SPLIT_emp3 \\ instantiate
     ) \\
     try_finally (
       (* CopyStrAw8 *)
